TypeSafety.v
@@ -1,74 +1,65 @@
-Require Import List Relations.
+From mathcomp Require Import all_ssreflect.
 Require Import Types Term Typing.
 Require Import Autosubst.Autosubst.
 
 Lemma typed_rename G t T :
   typed G t T ->
   forall G' r,
-  (forall x T, nth_error G x = Some T -> nth_error G' (r x) = Some T) ->
+  (forall d x, nth d G x = nth d G' (r x)) ->
   typed G' (rename r t) T.
 Proof.
-  induction 1; simpl; eauto.
-  - intros. constructor. apply IHtyped.
-    intros [ ]; eauto.
-  - intros. econstructor; eauto. apply IHtyped2.
-    intros [ ]; eauto.
+  induction 1 => /= ? ? Hnth; eauto.
+  - apply /typed_var => ?.
+    by rewrite -Hnth H.
+  - by apply /typed_abs /IHtyped => ? [ | ? ] /=.
+  - apply /typed_let; eauto.
+    by apply /IHtyped2 => ? [ | ? ] /=.
 Qed.
 
 Lemma typed_subst G t T :
   typed G t T ->
   forall s G',
-  (forall x T, nth_error G x = Some T -> typed G' (s x) T) ->
-  typed G' (t.[s]) T.
+  (forall x T, (forall d, nth d G x = T) -> typed G' (s x) T) ->
+  typed G' t.[s] T.
 Proof.
-  induction 1; simpl; eauto.
-  - intros. constructor. apply IHtyped.
-    unfold up. intros [ ]; simpl; inversion 1; eauto.
-    apply typed_rename with (G := G'); eauto.
-  - intros. econstructor; eauto. apply IHtyped2.
-    unfold up. intros [ ]; simpl; inversion 1; eauto.
-    apply typed_rename with (G := G'); eauto.
+  induction 1 => /= ? ? Hnth; eauto.
+  - apply /typed_abs /IHtyped => [ [ ? /(_ (typ_fvar 0)) /= -> | ? ? Hnth' ] /= ].
+    + exact /typed_var.
+    + exact /(typed_rename _ _ _ (Hnth _ _ Hnth')).
+  - apply /typed_let; eauto.
+    apply /IHtyped2 => [ [ ? /(_ (typ_fvar 0)) /= -> | ? ? Hnth' ] /= ].
+    + exact /typed_var.
+    + exact /(typed_rename _ _ _ (Hnth _ _ Hnth')).
 Qed.
 
 Lemma subject_reduction t t' :
   cbv t t' ->
-  forall G T, typed G t T ->
+  forall G T,
+  typed G t T ->
   typed G t' T.
 Proof.
   induction 1; inversion 1; subst; eauto.
   - inversion H4. subst.
-    apply typed_subst with (G := T1 :: G); eauto.
-    intros [ ]; simpl; inversion 1; subst; eauto.
-  - apply typed_subst with (G := T1 :: G); eauto.
-    intros [ ]; simpl; inversion 1; subst; eauto.
+    apply /typed_subst; eauto.
+    move => [ ? /(_ (typ_fvar 0)) <- // | /= ? ? ? ]; eauto.
+  - apply /typed_subst; eauto.
+    move => [ ? /(_ (typ_fvar 0)) <- // | /= ? ? ? ]; eauto.
 Qed.
 
-Lemma normal_arrow v T1 T2 :
+Lemma canonical_arrow v T1 T2 :
   value v ->
   typed nil v (typ_arrow T1 T2) ->
   exists t, v = trm_abs t.
-Proof. inversion 1. eauto. Qed.
+Proof. inversion 1; eauto. Qed.
 
-Lemma progress G t T :
-  typed G t T ->
-  G = nil ->
+Lemma progress t : forall T,
+  typed [::] t T ->
   value t \/ exists t', cbv t t'.
 Proof.
-  induction 1; intros; subst; eauto.
-  - destruct x; inversion H.
-  - destruct IHtyped1 as [ | [ ] ]; eauto.
-    edestruct normal_arrow; eauto. subst.
-    destruct IHtyped2 as [ | [ ] ]; eauto.
-  - destruct IHtyped1 as [ | [ ] ]; eauto.
-Qed.
-
-Theorem type_safety t t' T :
-  typed nil t T ->
-  clos_refl_trans_1n _ cbv t t' ->
-  value t' \/ exists t'', cbv t' t''.
-Proof.
-  induction 2.
-  - eapply progress; eauto.
-  - apply IHclos_refl_trans_1n.
-    eapply subject_reduction; eauto.
+  induction t; inversion 1; subst; eauto.
+  - move: (H2 (typ_fvar 0)).
+    by rewrite -(H2 (typ_bvar 0)) !nth_default.
+  - move: (IHt1 _ H3) => [ /((canonical_arrow _ _ _)^~H3) [ ? -> ] | [ ? ? ] ]; eauto.
+    move: (IHt2 _ H5) => [ ? | [ ? ? ] ]; eauto.
+  - move: (IHt _ H3) => [ ? | [ ? ? ] ]; eauto.
 Qed.
